theories/models/utp_ho2_pred.thy
@@ -3,25 +3,108 @@
 (* Author: Frank Zeyda, University of York                                    *)
 (******************************************************************************)
 theory utp_ho2_pred
-imports "../GLOBAL" "../generic/utp_generic" utp_ho2_value
+imports "../GLOBAL" "../generic/utp_generic" "../utils/utp_ho2_utils"
+  utp_ho2_value
 begin
 
 section {* HO2 Predicates *}
 
-text {*
-  Typing alone is not sufficient here; we require additional constraints for
-  consistency of higher-orderer variables at different levels.
+subsection {* Type Synonyms *}
 
-  This is work in progress!
-*}
+text {* Maybe these should be introduced as part of the instantiation. *}
+
+types STD_VAR = "STD_TYPE VAR"
+types HO1_VAR = "HO1_TYPE VAR"
+types HO2_VAR = "HO2_TYPE VAR"
+
+types STD_BINDING = "(STD_VALUE, STD_TYPE) BINDING"
+types HO1_BINDING = "(HO1_VALUE, HO1_TYPE) BINDING"
+types HO2_BINDING = "(HO2_VALUE, HO2_TYPE) BINDING"
+
+types STD_PREDICATE = "(STD_VALUE, STD_TYPE) ALPHA_PREDICATE"
+types HO1_PREDICATE = "(HO1_VALUE, HO1_TYPE) ALPHA_PREDICATE"
+types HO2_PREDICATE = "(HO2_VALUE, HO2_TYPE) ALPHA_PREDICATE"
+
+subsection {* HO2 Bindings *}
+
+definition HO2_CONSISTENT_1 :: "HO2_VAR \<Rightarrow> HO2_BINDING set" where
+"(IsProg2Var m2) \<longrightarrow>
+ HO2_CONSISTENT_1 m2 =
+   {b2 . (\<forall> b1 \<in> \<beta> (call (b2 m2)) .
+     (\<forall> m . (IsProgVar m) \<longrightarrow> b2 (m \<up>VAR) = (b1 m) \<up>VAL))}"
+
+definition HO2_CONSISTENT_2 :: "HO2_VAR \<Rightarrow> HO2_VAR \<Rightarrow> HO2_BINDING set" where
+"(IsProg1Var m1) \<and>
+ (IsProg2Var m2) \<and>
+ (var_name m1) = (var_name m2) \<longrightarrow>
+ HO2_CONSISTENT_2 m1 m2 =
+   {b2 . (\<forall> b1 \<in> \<beta> (call (b2 m2)) . (b1 \<down>BIND) \<in> \<beta> (call (b2 m1)))}"
+
+definition HO2_CONSISTENT :: "HO2_BINDING set" where
+"HO2_CONSISTENT =
+   (\<Inter> {bs . (\<exists> m2 . (IsProg2Var m2) \<and> bs = HO2_CONSISTENT_1 m2)}) \<inter>
+   (\<Inter> {bs . (\<exists> m1 m2 . (IsProg1Var m1) \<and> (IsProg2Var m2) \<and>
+     (var_name m1) = (var_name m2) \<and> bs = HO2_CONSISTENT_2 m1 m2)})"
+
+subsection {* Locale Instantiation *}
 
 locale HO2_PRED =
--- {* The mere use of the typed predicate locale is not appropriate for HO2. *}
-  HO2_VALUE_LOCALE + TYPED_PRED "ho2_type_rel"
+  HO2_VALUE_LOCALE +
+  GEN_PRED "(WT_BINDING ho2_type_rel) \<inter> HO2_CONSISTENT"
 
 interpretation HO2 : HO2_PRED
-apply (unfold HO2_PRED_def HO2_VALUE_LOCALE_def)
-apply (auto)
+apply (unfold HO2_PRED_def HO2_VALUE_LOCALE_def GEN_PRED_def)
+apply (simp add: HO2_CONSISTENT_def)
+apply (simp only: non_empty_exists)
+apply (rule_tac x =
+  "(\<lambda> v :: HO2_VAR .
+     if (IsStdVar v) then
+       (SOME x . ho2_type_rel x (type v))
+     else
+     if (IsProg1Var v) then
+       Prog1Val (Mk_STD_PREDICATE
+         (STD.FalseP (Dest_STD_ALPHABET (Prog1TypeOf (type v)))))
+     else
+     if (IsProg2Var v) then
+       Prog2Val (Mk_HO1_PREDICATE
+         (HO1.FalseP (Dest_HO1_ALPHABET (Prog2TypeOf (type v)))))
+     else dont_care)" in exI)
+apply (safe)
+-- {* Goal 1 *}
+apply (simp add: WT_BINDING)
+apply (safe, auto dest: IsVar_dest)
+-- {* Goal 1.1 *}
+apply (drule IsProg2Var_exists_type)
+apply (clarsimp)
+-- {* Goal 1.2 *}
+apply (drule IsProg1Var_exists_type)
+apply (clarsimp)
+-- {* Goal 1.3 *}
+apply (drule IsStdVar_exists_type)
+apply (clarsimp)
+apply (rule someI2_ex)
+apply (rule_tac x = "HO2_VALUE.BaseVal (SOME x . x : t)" in exI)
+apply (simp)
+apply (rule someI2_ex)
+apply (simp add: STD.type_non_empty)
+apply (assumption)+
+-- {* Goal 2 *}
+apply (simp add: HO2_CONSISTENT_1_def)
+apply (auto dest: IsVar_dest)
+-- {* Goal 2.1 *}
+apply (simp add: Call_simps)
+apply (simp add: HO1.FalseP_def)
+-- {* Goal 2.2 *}
+apply (simp add: Call_simps)
+apply (simp add: HO1.FalseP_def)
+-- {* Goal 2.3 *}
+apply (simp add: Call_simps)
+apply (simp add: HO1.FalseP_def)
+-- {* Goal 3 *}
+apply (simp add: HO2_CONSISTENT_2_def)
+apply (auto dest: IsVar_dest)
+apply (simp add: Call_simps)
+apply (simp add: HO1.FalseP_def)
 done
 
 subsection {* Semantic Domains *}
